finished all the proofs in LamYNmless.thy

Isabelle/LamYNmless.thy
@@ -82,7 +82,7 @@ where
 | red_R[intro]: "\<lbrakk> trm M ; N \<Rightarrow> N' \<rbrakk> \<Longrightarrow> App M N \<Rightarrow> App M N'"
 | abs[intro]: "\<lbrakk> finite L ; (\<And>x. x \<notin> L \<Longrightarrow> M^(FVar x) \<Rightarrow> M'^(FVar x)) \<rbrakk> \<Longrightarrow> Lam M \<Rightarrow> Lam M'"
 | beta[intro]: "\<lbrakk> trm (Lam M) ; trm N \<rbrakk> \<Longrightarrow> App (Lam M) N \<Rightarrow> M^N"
-| Y[intro]: "App (Y \<sigma>) M \<Rightarrow> App M (App (Y \<sigma>) M)"
+| Y[intro]: "trm M \<Longrightarrow> App (Y \<sigma>) M \<Rightarrow> App M (App (Y \<sigma>) M)"
 
 lemma test2: "Lam (App (Lam (BVar 0)) (FVar x)) \<Rightarrow> Lam (FVar x)"
 apply (rule_tac L="{}" in abs, simp, thin_tac "xa \<notin> {}")
@@ -134,6 +134,7 @@ case (1 L e k t)
   using "1"(3) "2" opn'_def by auto
 qed
 
+lemma opn_trm2: "trm e \<Longrightarrow> {k \<rightarrow> t}e = e" using opn_trm by simp
 
 
 lemma subst_open: "trm u \<Longrightarrow> ({n \<rightarrow> w}t)[x ::= u] = {n \<rightarrow> w [x ::= u]} (t [x ::= u])"
@@ -658,6 +659,526 @@ proof -
   using 1 assms apply simp+
   done
   thus ?thesis by auto
+qed
+
+inductive close :: "(ptrm \<Rightarrow> ptrm \<Rightarrow> bool) \<Rightarrow> ptrm \<Rightarrow> ptrm \<Rightarrow> bool" ("_* _  _" [80,80] 80) for R::"ptrm \<Rightarrow> ptrm \<Rightarrow> bool"
+where
+  base[intro]: "R a b \<Longrightarrow> R* a b"
+| refl[intro]: "R* a a"
+| trans[intro]: "\<lbrakk> R* a b ; R* b c \<rbrakk> \<Longrightarrow> R* a c"
+
+
+
+
+definition DP :: "(ptrm \<Rightarrow> ptrm \<Rightarrow> bool) \<Rightarrow> (ptrm \<Rightarrow> ptrm \<Rightarrow> bool) \<Rightarrow> bool" where
+"DP R T = (\<forall>a b c. R a b \<and> T a c \<longrightarrow> (\<exists>d. T b d \<and> R c d))"
+
+lemma DP_R_R_imp_DP_R_Rc_pbeta:
+  assumes "DP pbeta pbeta"
+    shows "DP pbeta (close pbeta)"
+using assms unfolding DP_def
+apply auto
+proof -
+case goal1 
+  from goal1(3,2) show ?case
+  apply (induct arbitrary: b rule:close.induct)
+  using goal1(1) by blast+
+qed
+
+lemma DP_R_R_imp_DP_Rc_Rc_pbeta:
+  assumes "DP pbeta pbeta"
+    shows "DP (close pbeta) (close pbeta)"
+using assms unfolding DP_def
+apply auto
+proof -
+case goal1 
+  from goal1(2,3) show ?case
+  apply (induct arbitrary: c rule:close.induct)
+  using DP_R_R_imp_DP_R_Rc_pbeta using DP_def assms apply fastforce
+  apply auto
+  by blast
+qed
+
+
+lemma trm_beta_Y_simp1: "M \<Rightarrow> M' \<Longrightarrow> trm M \<and> trm M'"
+apply rule
+apply (induct M' rule:beta_Y.induct)
+apply (subst trm.simps, simp)+
+apply auto[1]
+apply (simp add: lam trm.app)
+apply (simp add: trm.Y trm.app)
+apply (induct M M' rule:beta_Y.induct)
+apply (subst trm.simps, simp)+
+apply auto[1]
+apply (rule trm_opn)
+apply (simp add: lam)
+apply (simp add: trm.Y trm.app)
+done
+
+lemma pbeta_refl[intro]: "trm s \<Longrightarrow> s \<Rightarrow>\<parallel> s"
+apply (induct s rule:trm.induct)
+by auto
+
+
+lemma M1': "M \<Rightarrow> M' \<Longrightarrow> M \<Rightarrow>\<parallel> M'"
+proof (induct M M' rule:beta_Y.induct)
+case red_L 
+  show ?case
+  apply (rule pbeta.app)
+  using trm_beta_Y_simp1 red_L apply simp
+  apply (rule pbeta_refl)
+  using red_L by simp
+next
+case red_R 
+  show ?case
+  apply (rule pbeta.app)
+  apply (rule pbeta_refl)
+  using trm_beta_Y_simp1 red_R by auto
+next
+case (abs L) 
+  show ?case
+  apply (rule_tac L=L in pbeta.abs)
+  using abs by auto
+next
+case (beta M N)
+  from beta(1) obtain L where 1: "finite L" "\<forall>x. x \<notin> L \<longrightarrow> trm (M^FVar x)" using trm.simps by (metis finite.intros(1) trm_opn)
+  show ?case 
+  apply (rule_tac L=L in pbeta.beta)
+  using 1 apply simp
+  apply (rule pbeta_refl)
+  using 1 apply simp
+  apply (rule pbeta_refl)
+  using beta by simp
+next
+case Y thus ?case by auto
+qed
+
+lemma M1: "beta_Y* M M' \<Longrightarrow> pbeta* M M'"
+apply (induct M M' rule:close.induct)
+apply auto
+apply (rule base)
+by (simp add: M1')
+
+
+lemma red_r_close: "beta_Y* N N' \<Longrightarrow> trm M \<Longrightarrow> beta_Y* (App M N) (App M N')"
+apply (induct rule:close.induct)
+by auto
+
+lemma red_l_close: "beta_Y* M M' \<Longrightarrow> trm N \<Longrightarrow> beta_Y* (App M N) (App M' N)"
+apply (induct rule:close.induct)
+by auto
+
+lemma beta_Y_beta': "trm (Lam M) \<Longrightarrow> trm N \<Longrightarrow> App (Lam M) N \<Rightarrow> {0 \<rightarrow> N} M" using beta_Y.beta opn'_def by simp
+
+lemma Lem2_5_1'_beta_Y:
+  assumes "s \<Rightarrow> s'"
+      shows "(s[x ::= FVar y]) \<Rightarrow> (s'[x ::= FVar y])"
+using assms proof (induct s s' rule:beta_Y.induct)
+case (red_L N M M')
+  show ?case 
+  unfolding subst.simps
+  apply (rule beta_Y.red_L)
+  using red_L trm.var subst_trm by blast+
+next
+case (red_R M N N')
+  show ?case 
+  unfolding subst.simps
+  apply (rule beta_Y.red_R)
+  using red_R trm.var subst_trm by blast+
+next
+case (abs L M M') 
+  show ?case
+  unfolding subst.simps
+  apply (rule_tac L="L \<union> {x}" in beta_Y.abs)
+  using abs apply simp 
+  unfolding opn'_def
+  apply (subst subst_fresh2[where x=x and u="FVar y"])
+  apply auto[1]
+  apply (subst(8) subst_fresh2[where x=x and u="FVar y"])
+  apply auto[1]
+  apply (subst subst_open2)
+  defer
+  apply (subst subst_open2)
+  defer
+  defer
+  apply (rule trm.var)
+  using abs unfolding opn'_def
+  by simp
+ next
+case (beta M N)
+  show ?case unfolding subst.simps opn'_def
+  apply (subst subst_open)
+  apply (rule trm.var)
+  apply (rule beta_Y_beta')
+  defer
+  using beta trm.var subst_trm apply simp
+  using beta(1) trm.var subst_trm subst.simps(4) by metis
+next
+case Y 
+  show ?case unfolding subst.simps 
+  apply rule
+  using Y trm.var subst_trm by simp
+qed
+ 
+
+lemma beta_Y_lam_cls: "a \<Rightarrow> b \<Longrightarrow> Lam {0 <- x} a \<Rightarrow> Lam {0 <- x} b"
+apply (rule_tac L="{}" in beta_Y.abs)
+apply simp
+unfolding opn'_def
+defer
+apply (subst(2) cls_opn_eq_subst)
+using trm_beta_Y_simp1 apply simp
+apply (subst cls_opn_eq_subst)
+using trm_beta_Y_simp1 apply simp
+apply (rule Lem2_5_1'_beta_Y)
+by simp
+
+
+lemma abs_close: "\<lbrakk> \<And>x. x \<notin> L \<Longrightarrow> beta_Y* (M^FVar x) (M'^FVar x) ; finite L \<rbrakk> \<Longrightarrow> beta_Y* (Lam M) (Lam M')"
+proof goal_cases
+case 1
+  note 11 = 1
+  then obtain x where 2: "x \<notin> L \<union> FV M \<union> FV M'" by (meson FV_finite finite_UnI x_Ex)
+  with 1 have "op \<Rightarrow>* M^FVar x  M'^FVar x" by simp
+  then show ?case
+  apply (subst (4)fv_opn_cls_id2[where k=0 and x=x])
+  using 2 apply simp
+  apply (subst (2)fv_opn_cls_id2[where k=0 and x=x])
+  using 2 apply simp
+  unfolding opn'_def
+  apply (induct rule:close.induct)
+  apply auto
+  apply (rule base)
+  apply (rule beta_Y_lam_cls)
+  by simp
+qed
+
+
+lemma M2: "pbeta* M M' \<Longrightarrow> beta_Y* M M'"
+proof (induct M M' rule:close.induct)
+case refl show ?case by (rule close.refl)
+next
+case trans 
+  show ?case apply (rule close.trans)
+  using trans by simp+
+next
+case base thus ?case
+  proof (induct rule:pbeta.induct)
+  case refl show ?case by (rule close.refl)
+  next
+  case reflY show ?case by (rule close.refl)
+  case (app M M' N N') 
+    show ?case
+    apply (rule_tac b="App M N'" in close.trans)
+    using red_r_close app.hyps(1,4) trm_pbeta_simp1 apply auto[1]
+    using red_l_close app.hyps(2,3) trm_pbeta_simp1 by blast
+  next
+  case (abs L M M')
+    show ?case
+    apply (rule_tac L=L in  abs_close)
+    using abs by simp+
+  next
+  case (beta L M M' N N')
+    show ?case
+    apply (rule_tac b="App (Lam M') N" in close.trans)
+    apply (rule red_l_close)
+    apply (rule_tac L=L in  abs_close)
+    using beta apply simp
+    using beta trm_pbeta_simp1 apply simp+
+    apply (rule_tac b="App (Lam M') N'" in close.trans)
+    apply (rule red_r_close)
+    using beta apply simp
+    apply (rule_tac L=L in trm.lam)
+    using beta apply simp
+    using beta(2) trm_pbeta_simp1 apply auto[1]
+    apply (rule close.base)
+    apply (rule beta_Y.beta)
+    apply (rule_tac L=L in trm.lam)
+    using beta apply simp
+    using beta(2) trm_pbeta_simp1 apply auto[1]
+    using beta trm_pbeta_simp1 by simp
+  next
+  case (Y M M' \<sigma>) 
+    show ?case
+    apply (rule_tac b="App M (App (Y \<sigma>) M)" in close.trans)
+    apply (rule close.base)
+    apply (rule beta_Y.Y)
+    using Y trm_pbeta_simp1 apply simp
+    apply (rule_tac b="App M' (App (Y \<sigma>) M)" in close.trans)
+    apply (rule red_l_close)
+    using Y apply simp
+    using Y trm_pbeta_simp1 apply auto[1]
+    apply (rule red_r_close)
+    apply (rule red_r_close)
+    using Y trm_pbeta_simp1 by auto
+  qed
+qed
+
+
+lemma wf_ctxt_cons: "wf_ctxt ((x, \<sigma>)#\<Gamma>) \<Longrightarrow> wf_ctxt \<Gamma> \<and> x \<notin> fst`set \<Gamma>"
+apply (cases rule:wf_ctxt.cases)
+by auto
+
+lemma wt_terms_impl_wf_ctxt: "\<Gamma> \<turnstile> M : \<sigma> \<Longrightarrow> wf_ctxt \<Gamma>"
+apply (induct rule:wt_trm.induct)
+apply auto
+using wf_ctxt_cons by (meson x_Ex)
+
+
+lemma subst_typ_aux: "(x, \<tau>) # \<Gamma> \<turnstile> FVar y : \<sigma> \<Longrightarrow> x = y \<Longrightarrow> \<tau> = \<sigma>"
+proof (rule ccontr, goal_cases)
+case 1 
+  then have "wf_ctxt ((y, \<tau>) # \<Gamma>)" by (simp add: wt_terms_impl_wf_ctxt)
+  then have "y \<notin> fst`set \<Gamma>" by (simp add: wf_ctxt_cons)
+  then have "(y, \<sigma>) \<notin> set \<Gamma>" by force
+  with 1(3) have 2: "(y, \<sigma>) \<notin> set ((y, \<tau>) # \<Gamma>)" by simp
+  from 1(1) have "(y, \<sigma>) \<in> set ((y, \<tau>) # \<Gamma>)" apply (cases rule:wt_trm.cases) by auto
+  with 2 show ?case by simp
+qed
+
+lemma weakening:
+  fixes \<Gamma> \<Gamma>' M \<sigma>
+  assumes "\<Gamma> \<turnstile> M : \<sigma>" and "set \<Gamma> \<subseteq> set \<Gamma>'"
+  and "wf_ctxt \<Gamma>'"
+  shows "\<Gamma>' \<turnstile> M : \<sigma>"
+using assms proof (induct \<Gamma> M \<sigma> arbitrary:\<Gamma>' rule:wt_trm.induct)
+case var 
+  show ?case 
+  apply (rule wt_trm.var) 
+  using var by auto
+next
+case app
+  show ?case
+  apply (rule wt_trm.app)
+  using app by auto
+next
+case (abs L \<sigma> \<Gamma> t \<tau>)
+  have 1: "\<And>x. x \<notin> (L \<union> fst ` set \<Gamma>') \<Longrightarrow> wf_ctxt ((x, \<sigma>) # \<Gamma>')"
+  apply (rule cons)
+  using abs by simp+
+
+  show ?case
+  apply (rule_tac L="L \<union> fst ` set \<Gamma>'" in wt_trm.abs)
+  using abs apply simp
+  apply (rule abs(3))
+  apply simp
+  using abs.prems(1) 1 by auto
+next
+case Y thus ?case using wt_trm.Y by simp
+qed
+
+lemma wf_ctxt_exchange: "wf_ctxt ((x,\<sigma>) # (y,\<pi>) # \<Gamma>) \<Longrightarrow> wf_ctxt ((y,\<pi>) # (x,\<sigma>) # \<Gamma>)"
+proof goal_cases
+case 1 
+  then have "wf_ctxt ((y,\<pi>) # \<Gamma>) \<and> x \<notin> fst`set ((y,\<pi>) # \<Gamma>)" by (rule wf_ctxt_cons)
+  then have 1: "wf_ctxt ((y,\<pi>) # \<Gamma>)" "x \<notin> fst`set ((y,\<pi>) # \<Gamma>)"  by simp+
+  from 1(1) have 2: "wf_ctxt \<Gamma> \<and> y \<notin> fst`set \<Gamma>" by (rule wf_ctxt_cons)
+  from 1(2) have 3: "x \<notin> fst`set \<Gamma>" by simp
+  from 1(2) 2 have 4: "y \<notin> fst`set((x,\<sigma>) # \<Gamma>)" by auto
+
+  show ?case
+  apply (rule cons)
+  using 4 apply simp  
+  apply (rule cons)
+  using 3 apply simp
+  using 2 by simp
+qed
+
+lemma exchange: "(x,\<sigma>) # (y,\<pi>) # \<Gamma> \<turnstile> M : \<delta> \<Longrightarrow> (y,\<pi>) # (x,\<sigma>) # \<Gamma> \<turnstile> M : \<delta>"
+proof goal_cases
+case 1
+  have "set ((x,\<sigma>) # (y,\<pi>) # \<Gamma>) \<subseteq> set ((y,\<pi>) # (x,\<sigma>) # \<Gamma>)" by auto
+  thus ?case using 1 weakening wt_terms_impl_wf_ctxt wf_ctxt_exchange by blast
+qed
+
+(*thm wt_trm.cases
+lemma wt_trm_cases_2:
+  shows "\<Gamma> \<turnstile> Lam. M : a3 \<Longrightarrow> atom x \<sharp> \<Gamma>\<Longrightarrow> (\<And>\<sigma> \<tau>. a3 = \<sigma> \<rightarrow> \<tau> \<Longrightarrow> ((x, \<sigma>)#\<Gamma>) \<turnstile> M : \<tau> \<Longrightarrow> P) \<Longrightarrow> P"
+*)
+
+lemma trm_wt_trm: "\<Gamma> \<turnstile> M : \<sigma> \<Longrightarrow> trm M"
+apply (induct \<Gamma> M \<sigma> rule:wt_trm.induct)
+apply (subst trm.simps, simp)+
+apply auto[1]
+by (subst trm.simps, simp)+
+
+
+
+lemma subst_typ':
+  assumes "trm M" and "((x,\<tau>)#\<Gamma>) \<turnstile> M : \<sigma>" and "\<Gamma> \<turnstile> N : \<tau>"
+  shows "\<Gamma> \<turnstile> M[x ::= N] : \<sigma>"
+using assms proof (induct M arbitrary: \<Gamma> x N \<sigma> rule: trm.induct)
+case (var y)
+  show ?case
+  proof (cases "x = y")
+  case True 
+    show ?thesis 
+    apply (simp add: True)
+    using var subst_typ_aux True by blast
+  next
+  case False
+    from var have 1: "wf_ctxt \<Gamma>" using wt_terms_impl_wf_ctxt wf_ctxt_cons by auto
+    from var have "(y,\<sigma>) \<in> set ((x, \<tau>) # \<Gamma>)" apply (cases rule:wt_trm.cases) by auto
+    with False have 2: "(y,\<sigma>) \<in> set \<Gamma>" by simp
+
+    show ?thesis
+    using False apply simp
+    apply (rule_tac wt_trm.var)
+    using 1 2 by simp+
+  qed
+next
+case (app M' N')
+  from app(5) obtain \<pi> where  "(x, \<tau>) # \<Gamma> \<turnstile> M' : \<pi> \<rightarrow> \<sigma>" "(x, \<tau>) # \<Gamma> \<turnstile> N' : \<pi>" 
+    by (cases rule:wt_trm.cases, simp)
+  with app(2,4,6) have ih: "\<Gamma> \<turnstile> M'[x ::= N] : \<pi> \<rightarrow> \<sigma>" "\<Gamma> \<turnstile> N'[x ::= N] : \<pi>" by simp+
+  show ?case
+  unfolding subst.simps
+  apply (rule wt_trm.app)
+  using ih by simp+
+next
+case (lam L M)
+  from lam(4) obtain \<pi> \<delta> where 1: "\<sigma> = \<pi> \<rightarrow> \<delta>" "(x, \<tau>) # \<Gamma> \<turnstile> Lam M : \<pi> \<rightarrow> \<delta>" by (cases rule:wt_trm.cases, simp)
+  
+  from 1(2) have "\<exists>L. finite L \<and> (\<forall>x'. x' \<notin> L \<longrightarrow> (x', \<pi>) # (x, \<tau>) # \<Gamma> \<turnstile> M^FVar x' : \<delta>)"
+  apply (drule_tac subst[OF wt_trm.simps])
+  by simp
+  then obtain L' where 2: "finite L'" "\<And>x'. x' \<notin> L' \<Longrightarrow> (x', \<pi>) # (x, \<tau>) # \<Gamma> \<turnstile> M^FVar x' : \<delta>" by auto                                                         
+  from 2(2) have 3: "\<And>x'. x' \<notin> L' \<Longrightarrow> (x, \<tau>) # (x', \<pi>) # \<Gamma> \<turnstile> M^FVar x' : \<delta>" by (rule exchange)
+
+  show ?case apply (subst subst.simps)
+  unfolding 1(1)
+  apply (rule_tac L="L \<union> L' \<union> {x} \<union> fst ` set \<Gamma>" in wt_trm.abs)
+  using lam 2 apply simp
+  apply (subst subst_open_var2)
+  using trm_wt_trm lam apply simp
+  apply auto[1]
+  apply (rule lam(3))
+  apply simp
+  apply (rule 3)
+  apply simp
+  apply (rule weakening)
+  using lam apply simp
+  apply auto[1]
+  apply (rule wf_ctxt.cons)
+  apply simp
+  using lam wt_terms_impl_wf_ctxt by simp
+next
+case (Y \<gamma>)
+  from Y(1) have 1: "\<sigma> = (\<gamma> \<rightarrow> \<gamma>) \<rightarrow> \<gamma>" by (cases rule:wt_trm.cases, simp)
+  show ?case unfolding subst.simps 1
+  apply (rule wt_trm.Y)
+  using Y wt_terms_impl_wf_ctxt wf_ctxt_cons by simp
+qed
+
+
+lemma subst_typ:
+  fixes L
+  assumes "finite L" "\<And>x. x \<notin> L \<Longrightarrow> ((x,\<tau>)#\<Gamma>) \<turnstile> M^FVar x : \<sigma>" and "\<Gamma> \<turnstile> N : \<tau>"
+  shows "\<Gamma> \<turnstile> M^N : \<sigma>"
+proof -
+  obtain x where 1: "x \<notin> L \<union> FV M" using assms by (meson FV_finite finite_UnI x_Ex)
+  with assms have 2: "((x,\<tau>)#\<Gamma>) \<turnstile> M^FVar x : \<sigma>" by simp
+
+  show ?thesis
+  apply (subst subst_intro2[where x=x])
+  apply (rule trm_wt_trm)
+  using assms apply simp
+  using 1 apply simp
+  apply (rule subst_typ')
+  apply (rule trm_wt_trm)
+  using 2 apply simp
+  apply (rule assms(2))
+  using 1 apply simp
+  using assms by simp
+qed
+
+
+lemma beta_Y_typ:
+  assumes "\<Gamma> \<turnstile> M : \<sigma>"
+  and "M \<Rightarrow> M'"
+  shows "\<Gamma> \<turnstile> M' : \<sigma>"
+using assms(2,1)
+proof (induct  M M' arbitrary: \<Gamma> \<sigma> rule: beta_Y.induct)
+case (red_L N M M')
+  from red_L(4) obtain \<tau> where 1: "\<Gamma> \<turnstile> M : \<tau> \<rightarrow> \<sigma>" "\<Gamma> \<turnstile> N : \<tau>"
+    apply (cases rule:wt_trm.cases) by simp
+  with red_L(3) have "\<Gamma> \<turnstile> M' : \<tau> \<rightarrow> \<sigma>" by simp
+  thus ?case 
+    apply (rule wt_trm.app)
+    using 1 by simp
+next
+case (red_R M N N')
+  from red_R(4) obtain \<tau> where 1: "\<Gamma> \<turnstile> M : \<tau> \<rightarrow> \<sigma>" "\<Gamma> \<turnstile> N : \<tau>"
+    apply (cases rule:wt_trm.cases) by simp
+  with red_R(3) have 2: "\<Gamma> \<turnstile> N' : \<tau>" by simp
+  show ?case 
+    apply (rule wt_trm.app)
+    using 1 2 by simp+
+next
+case (abs L M M')
+  from abs(4) obtain \<pi> \<tau> where 1: "\<sigma> = \<pi> \<rightarrow> \<tau>" "\<Gamma> \<turnstile> Lam M : \<pi> \<rightarrow> \<tau>"
+    apply (cases rule:wt_trm.cases) using abs.prems by blast
+  from 1(2) have "\<exists>L. finite L \<and> (\<forall>x. x \<notin> L \<longrightarrow> (x, \<pi>) # \<Gamma> \<turnstile> M^FVar x : \<tau>)"
+  apply (drule_tac subst[OF wt_trm.simps])
+  by simp
+  then obtain L' where 2: "finite L'" "\<And>x. x \<notin> L' \<Longrightarrow> (x, \<pi>) # \<Gamma> \<turnstile> M^FVar x : \<tau>" by auto
+
+  have 3: "\<And>x. x \<notin> L \<union> L' \<Longrightarrow> ((x,\<pi>)#\<Gamma>) \<turnstile> M'^FVar x : \<tau>"
+  apply (rule abs(3))
+  using 2 by auto
+
+  show ?case
+    apply (subst 1(1))
+    apply (rule_tac L="L \<union> L'" in wt_trm.abs)
+    using abs 2 3 by simp+
+next
+case (beta M N) 
+  from beta(3) obtain \<tau> where 1: "\<Gamma> \<turnstile> (Lam M) : \<tau> \<rightarrow> \<sigma>" "\<Gamma> \<turnstile> N : \<tau>" 
+    apply (cases rule:wt_trm.cases) by simp
+  from 1(1) have 2: "\<exists>L. finite L \<and> (\<forall>x. x \<notin> L \<longrightarrow> (x, \<tau>) # \<Gamma> \<turnstile> M^FVar x : \<sigma>)"
+  apply (drule_tac subst[OF wt_trm.simps])
+  by simp
+  then obtain L where 3: "finite L" "\<And>x. x \<notin> L \<Longrightarrow> (x, \<tau>) # \<Gamma> \<turnstile> M^FVar x : \<sigma>" by auto
+
+  show ?case
+  apply (rule_tac L=L in subst_typ)
+  using 3 1(2) by auto
+next
+case (Y M \<tau>)
+  from Y(2) obtain \<pi> where 1: "\<Gamma> \<turnstile> (Y \<tau>) : \<pi> \<rightarrow> \<sigma>" "\<Gamma> \<turnstile> M : \<pi>" 
+    apply (cases rule:wt_trm.cases) by simp
+  have "\<Gamma> \<turnstile> (Y \<tau>) : (\<tau> \<rightarrow> \<tau>) \<rightarrow> \<tau>" apply (rule wt_trm.Y)
+    using wt_terms_impl_wf_ctxt Y by simp
+  with 1(1) have "\<pi> \<rightarrow> \<sigma> = (\<tau> \<rightarrow> \<tau>) \<rightarrow> \<tau>" apply (cases rule:wt_trm.cases) by simp
+  then have 2: "\<pi> = \<tau> \<rightarrow> \<tau>" "\<sigma> = \<tau>" by simp+
+  show ?case
+    apply (subst 2)
+    apply (rule wt_trm.app)
+    defer
+    apply (rule wt_trm.app)
+    apply (rule wt_trm.Y)
+    using wt_terms_impl_wf_ctxt Y apply simp
+    using 1(2) 2(1) by simp+
+qed
+
+lemma beta_Y_c_typ:
+  assumes "\<Gamma> \<turnstile> M : \<sigma>"
+  and "beta_Y* M M'"
+  shows "\<Gamma> \<turnstile> M' : \<sigma>"
+using assms(2,1)
+apply (induct M M' arbitrary: \<sigma> rule: close.induct)
+using beta_Y_typ by auto
+
+
+lemma church_rosser_typ:
+  assumes "\<Gamma> \<turnstile> a : \<sigma>"
+      and "beta_Y* a b"
+      and "beta_Y* a c"
+    shows "\<exists>d. beta_Y* b d \<and> beta_Y* c d \<and> \<Gamma> \<turnstile> d : \<sigma>"
+proof -
+  from assms have "pbeta* a b" "pbeta* a c" using M1 base by simp+
+  then obtain d where "pbeta* b d" "pbeta* c d" by (metis DP_R_R_imp_DP_Rc_Rc_pbeta DP_def Lem2_5_2) 
+  thus ?thesis using M2 beta_Y_c_typ assms by blast
 qed
 
 end
